StmtRelML.thy
@@ -32,60 +32,34 @@ ML \<open>
     resolve_tac ctxt [@{thm red_ast_bpl_refl}] THEN'
     assume_tac ctxt
 
-  fun red_assign_tac ctxt exp_wf_rel_info (exp_rel_info : exp_rel_info) var_context_vpr_tac var_rel_tac lookup_bpl_target_thm =
-    (Rmsg' "Assign1" (resolve_tac ctxt [@{thm assign_rel_simple[where ?Trep=ty_repr_basic]}]) ctxt) THEN'
-    (Rmsg' "Assign2" (assm_full_simp_solved_with_thms_tac [] ctxt) ctxt) THEN'
-    (Rmsg' "Assign3" (var_context_vpr_tac ctxt |> SOLVED') ctxt) THEN'
-    
-    (* well-def RHS *)
-    (* begin *)
-    (Rmsg' "Assign4" (resolve_tac ctxt [@{thm wf_rel_extend_1}]) ctxt) THEN'
-    (Rmsg' "Assign Wf RHS" (exp_wf_rel_non_trivial_tac exp_wf_rel_info exp_rel_info ctxt |> SOLVED') ctxt) THEN'
-    (Rmsg' "Assign5" (progress_tac ctxt) ctxt) THEN'
-    (* end *)
-    
-    (Rmsg' "Assign6" (assm_full_simp_solved_with_thms_tac [lookup_bpl_target_thm] ctxt) ctxt) THEN'
-    (Rmsg' "Assign7" (assm_full_simp_solved_with_thms_tac [] ctxt) ctxt) THEN' 
-    
-    (* prove updated Viper and Boogie states are still in relation *)
-    (* begin *)
-    (Rmsg' "Assign8" (resolve_tac ctxt [@{thm state_rel_store_update_2}]) ctxt) THEN'
-    (Rmsg' "Assign9" (assm_full_simp_solved_with_thms_tac [] ctxt) ctxt) THEN'
-    (Rmsg' "Assign10" (assm_full_simp_solved_with_thms_tac [] ctxt) ctxt) THEN'
-    (Rmsg' "Assign11" (assm_full_simp_solved_with_thms_tac [] ctxt) ctxt) THEN'
-    (Rmsg' "Assign12" (var_rel_tac ctxt |> SOLVED') ctxt) THEN'
-    (Rmsg' "Assign13" (assm_full_simp_solved_with_thms_tac [] ctxt) ctxt) THEN'
-    (Rmsg' "Assign14" (assm_full_simp_solved_with_thms_tac [lookup_bpl_target_thm] ctxt) ctxt) THEN'
-    (Rmsg' "Assign15" (assm_full_simp_solved_with_thms_tac [] ctxt) ctxt) THEN'
-    (* end *)
-        
-    (Rmsg' "Assign16" (assm_full_simp_solved_with_thms_tac @{thms type_interp_rel_wf_vbpl_no_domains ty_repr_basic_def} ctxt) ctxt) THEN'
-    (Rmsg' "Assign17" (exp_rel_tac exp_rel_info ctxt |> SOLVED') ctxt)
-
-  datatype stmt_rel_hint = 
-    AssignHint of 
-       exp_wf_rel_info *
-       exp_rel_info * (* for relating RHS of assignment *)
-       thm (* lookup target theorem *) 
-  | SeqnHint of stmt_rel_hint list
+  datatype 'a stmt_rel_hint = 
+    AtomicHint of 'a 
+  | SeqnHint of ('a stmt_rel_hint) list
   | IfHint of 
        exp_wf_rel_info *       
        exp_rel_info *
-       stmt_rel_hint * (* thn branch *)
-       stmt_rel_hint
-  | NoHint (* used for debugging purposes *)
-              
+       ('a stmt_rel_hint) * (* thn branch *)
+       ('a stmt_rel_hint)   (* els branch *)
+  | NoHint (* used for debugging purposes *) 
+     
 
-  type stmt_rel_info = {
+  type basic_stmt_rel_info = {
       ctxt_wf_thm: thm,
       tr_def_thm: thm,
       var_rel_tac: (Proof.context -> int -> tactic),
-      var_context_vpr_tac: (Proof.context -> int -> tactic)
- }
-  
+      var_context_vpr_tac: (Proof.context -> int -> tactic),
+      field_rel_single_tac : (Proof.context -> int -> tactic), 
+      type_interp_econtext: thm  
+  }
 
+  type 'a atomic_rel_tac = (Proof.context -> basic_stmt_rel_info -> 'a -> int -> tactic)
 
- fun stmt_rel_tac ctxt (info: stmt_rel_info) stmt_rel_hint =
+  type 'a stmt_rel_info = {
+    basic_stmt_rel_info: basic_stmt_rel_info,
+    atomic_rel_tac: 'a atomic_rel_tac
+  }
+
+ fun stmt_rel_tac ctxt (info: 'a stmt_rel_info)(stmt_rel_hint: 'a stmt_rel_hint) =
     case stmt_rel_hint of 
        SeqnHint [] => resolve_tac ctxt [@{thm stmt_rel_skip}]
     |  SeqnHint [_] => error "SeqnHint with single node appears"
@@ -93,25 +67,21 @@ ML \<open>
     | _ => stmt_rel_single_stmt_tac ctxt info stmt_rel_hint
 and
      stmt_rel_tac_seq _ _ [] = K all_tac
-   | stmt_rel_tac_seq ctxt (info: stmt_rel_info) [h] =
+   | stmt_rel_tac_seq ctxt (info: 'a stmt_rel_info) [h] =
        stmt_rel_tac ctxt info h
-   | stmt_rel_tac_seq ctxt (info: stmt_rel_info) (h1 :: h2 :: hs) = 
+   | stmt_rel_tac_seq ctxt (info: 'a stmt_rel_info) (h1 :: h2 :: hs) = 
        resolve_tac ctxt [@{thm stmt_rel_seq_same_rel}] THEN'
        stmt_rel_tac ctxt info h1 THEN'
        stmt_rel_tac_seq ctxt info (h2 :: hs)
 and 
      stmt_rel_single_stmt_tac _ _ NoHint = K all_tac
-   | stmt_rel_single_stmt_tac ctxt (info: stmt_rel_info) hint_hd =
+   | stmt_rel_single_stmt_tac ctxt (info: 'a stmt_rel_info) hint_hd =
     (* Each statement associated with a hint is translated by the actual encoding followed by 
        \<open>assume state(Heap, Mask)\<close>. This is why we apply a propagation rule first. *)
     resolve_tac ctxt [@{thm stmt_rel_propagate_2_same_rel}] THEN'
     (
       case hint_hd of
-        AssignHint (exp_wf_rel_info, exp_rel_info, lookup_bpl_target_thm) => 
-               red_assign_tac ctxt exp_wf_rel_info exp_rel_info 
-                        (#var_context_vpr_tac info) 
-                        (#var_rel_tac info) 
-                        lookup_bpl_target_thm
+        AtomicHint a => (#atomic_rel_tac info) ctxt (#basic_stmt_rel_info info) a
       | IfHint (exp_wf_rel_info, exp_rel_info, thn_hint, els_hint) =>
            (Rmsg' "If0" (resolve_tac ctxt [@{thm stmt_rel_if}]) ctxt) THEN'
            (
@@ -141,7 +111,114 @@ and
       | _ => error "unsupported hint in stmt_rel_single_stmt_tac"
     ) THEN'
     (* now reduce \<open>assume state(Heap, Mask)\<close> *)
-    progress_assume_good_state_tac ctxt (#ctxt_wf_thm info) (#tr_def_thm info)  
+    progress_assume_good_state_tac ctxt (#ctxt_wf_thm (#basic_stmt_rel_info info)) (#tr_def_thm (#basic_stmt_rel_info info))
+\<close>
+
+ML \<open>
+
+  datatype atomic_rel_hint = 
+     AssignHint of 
+       exp_wf_rel_info *
+       exp_rel_info * (* for relating RHS of assignment *)
+       thm (* lookup target theorem *)
+  | FieldAssignHint of
+       exp_wf_rel_info * (* well-definedness receiver *)
+       exp_wf_rel_info * (* well-definedness rhs *)
+       exp_rel_info * (* receiver *)
+       exp_rel_info   (* rhs *)
+
+  fun red_assign_tac ctxt (basic_stmt_rel_info : basic_stmt_rel_info) exp_wf_rel_info (exp_rel_info : exp_rel_info) lookup_bpl_target_thm =
+    (* TODO     (Rmsg' "Assign1" (resolve_tac ctxt [@{thm assign_rel_simple[where ?Trep=ty_repr_basic]}]) ctxt) THEN' *)
+    (Rmsg' "Assign1" (resolve_tac ctxt [@{thm assign_rel_simple}]) ctxt) THEN'
+    (Rmsg' "Assign2" (assm_full_simp_solved_with_thms_tac [] ctxt) ctxt) THEN'
+    (Rmsg' "Assign3" ((#var_context_vpr_tac basic_stmt_rel_info) ctxt |> SOLVED') ctxt) THEN'
+    (Rmsg' "Assign3b" (simp_only_tac [#type_interp_econtext basic_stmt_rel_info] ctxt THEN'
+                        resolve_tac ctxt @{thms type_interp_rel_wf_vbpl_basic}) ctxt) THEN'
+    
+    (* well-def RHS *)
+    (* begin *)
+    (Rmsg' "Assign4" (resolve_tac ctxt [@{thm wf_rel_extend_1}]) ctxt) THEN'
+    (Rmsg' "Assign Wf RHS" (exp_wf_rel_non_trivial_tac exp_wf_rel_info exp_rel_info ctxt |> SOLVED') ctxt) THEN'
+    (Rmsg' "Assign5" (progress_tac ctxt) ctxt) THEN'
+    (* end *)
+    
+    (Rmsg' "Assign6" (assm_full_simp_solved_with_thms_tac [lookup_bpl_target_thm] ctxt) ctxt) THEN'
+    (Rmsg' "Assign7" (assm_full_simp_solved_with_thms_tac [] ctxt) ctxt) THEN' 
+    
+    (* prove updated Viper and Boogie states are still in relation *)
+    (* begin *)
+    (Rmsg' "Assign8" (resolve_tac ctxt [@{thm state_rel_store_update_2}]) ctxt) THEN'
+    (Rmsg' "Assign9" (assm_full_simp_solved_with_thms_tac [] ctxt) ctxt) THEN'
+    (Rmsg' "Assign10" (assm_full_simp_solved_with_thms_tac [] ctxt) ctxt) THEN'
+    (Rmsg' "Assign11" (assm_full_simp_solved_with_thms_tac [] ctxt) ctxt) THEN'
+    (Rmsg' "Assign12" ( (#var_rel_tac basic_stmt_rel_info) ctxt |> SOLVED') ctxt) THEN'
+    (Rmsg' "Assign13" (assm_full_simp_solved_with_thms_tac [] ctxt) ctxt) THEN'
+    (Rmsg' "Assign14" (assm_full_simp_solved_with_thms_tac [lookup_bpl_target_thm] ctxt) ctxt) THEN'
+    (Rmsg' "Assign15" (assm_full_simp_solved_with_thms_tac [] ctxt) ctxt) THEN'
+    (* end *)
+        
+    (Rmsg' "Assign16" (exp_rel_tac exp_rel_info ctxt |> SOLVED') ctxt)
+
+
+  fun field_rel_single_inst_tac field_rel_tac field_lookup_tac ctxt =
+    resolve_tac ctxt [@{thm field_rel_single_intro}] THEN'
+    field_lookup_tac ctxt THEN'
+    (assm_full_simp_solved_with_thms_tac @{thms ty_repr_basic_def} ctxt) THEN'
+    field_rel_tac ctxt THEN'
+    assm_full_simp_solved_with_thms_tac [] ctxt
+
+  fun wf_writeable_field_rel_tac rcv_exp_rel_info (basic_stmt_rel_info : basic_stmt_rel_info) ctxt =
+     (* need to first progress the configuration in case the currently active bigblock is not unfolded or
+        if the current bigblock is empty *)
+     resolve_tac ctxt [@{thm wf_rel_extend_2}] THEN' 
+     progress_tac ctxt THEN'
+     (Rmsg' "WfWriteableField1" (resolve_tac ctxt [@{thm syn_field_access_writeable_wf_rel} OF 
+                                                     [#ctxt_wf_thm basic_stmt_rel_info, @{thm wf_ty_repr_basic}]
+                                                  ]) ctxt) THEN'
+     (Rmsg' "WfWriteableField2" (assm_full_simp_solved_with_thms_tac [] ctxt) ctxt) THEN'
+     (Rmsg' "WfWriteableField3" (assm_full_simp_solved_with_thms_tac [#tr_def_thm basic_stmt_rel_info, @{thm read_mask_concrete_def}] ctxt) ctxt) THEN'
+     (Rmsg' "WfWriteableField4" (simp_tac_with_thms [#tr_def_thm basic_stmt_rel_info] ctxt) ctxt) THEN'     
+     (Rmsg' "WfWriteableField5" (resolve_tac ctxt [@{thm mask_read_wf_concrete} OF 
+                                                     [#ctxt_wf_thm basic_stmt_rel_info, @{thm wf_ty_repr_basic}]
+                                                  ]) ctxt) THEN'
+     (Rmsg' "WfWriteableField6" (assm_full_simp_solved_with_thms_tac [#tr_def_thm basic_stmt_rel_info] ctxt) ctxt) THEN'
+     (Rmsg' "WfWriteableField7 (exp rel rcv)" (exp_rel_tac rcv_exp_rel_info ctxt) ctxt) THEN'
+     (Rmsg' "WfWriteableField8" (assm_full_simp_solved_with_thms_tac [#tr_def_thm basic_stmt_rel_info] ctxt) ctxt) THEN'
+     (Rmsg' "WfWriteableField9 (single field rel)" ((#field_rel_single_tac basic_stmt_rel_info) ctxt) ctxt) THEN'
+     (Rmsg' "WfWriteableField10" (assm_full_simp_solved_with_thms_tac @{thms ty_repr_basic_def} ctxt) ctxt)
+
+     
+
+  fun field_assign_rel_tac ctxt (basic_stmt_rel_info : basic_stmt_rel_info) atomic_hint =
+    (case atomic_hint of 
+       FieldAssignHint (rcv_wf_rel_info, rhs_wf_rel_info, rcv_exp_rel_info, rhs_exp_rel_info) =>
+       (Rmsg' "FieldAssign1" (resolve_tac ctxt [@{thm field_assign_rel_inst[OF wf_ty_repr_basic]}]) ctxt) THEN'
+       (Rmsg' "FieldAssign2" (assm_full_simp_solved_with_thms_tac [] ctxt) ctxt) THEN'
+       (Rmsg' "FieldAssign3" (simp_tac_with_thms [#tr_def_thm basic_stmt_rel_info] ctxt THEN'
+                              resolve_tac ctxt [@{thm heap_update_wf_concrete} OF [#ctxt_wf_thm basic_stmt_rel_info, @{thm wf_ty_repr_basic}]])
+                               ctxt) THEN'
+       (Rmsg' "FieldAssign4" (assm_full_simp_solved_with_thms_tac @{thms ty_repr_basic_def} ctxt) ctxt) THEN'
+       (Rmsg' "FieldAssign5" (assm_full_simp_solved_with_thms_tac [] ctxt) ctxt) THEN'
+       (Rmsg' "FieldAssign6" (assm_full_simp_solved_with_thms_tac [] ctxt) ctxt) THEN'
+       (* TODO: need to use wf_rel_extend *)
+       (Rmsg' "FieldAssign7 (Wf Rcv)" (exp_wf_rel_non_trivial_tac rcv_wf_rel_info rcv_exp_rel_info ctxt) ctxt) THEN'
+       (Rmsg' "FieldAssign8 (Wf Rhs)" (exp_wf_rel_non_trivial_tac rhs_wf_rel_info rhs_exp_rel_info ctxt) ctxt) THEN'
+       (Rmsg' "FieldAssign9 (Wf Writeable Field)" (wf_writeable_field_rel_tac rcv_exp_rel_info basic_stmt_rel_info ctxt) ctxt) THEN'
+       (Rmsg' "FieldAssign10" (assm_full_simp_solved_with_thms_tac [#tr_def_thm basic_stmt_rel_info] ctxt) ctxt) THEN'
+       (Rmsg' "FieldAssign11" (assm_full_simp_solved_with_thms_tac [#tr_def_thm basic_stmt_rel_info, @{thm update_heap_concrete_def}, @{thm ty_repr_basic_def}] ctxt) ctxt) THEN'
+       (Rmsg' "FieldAssign12 (Exp Rel Rcv)" (exp_rel_tac rcv_exp_rel_info ctxt) ctxt) THEN'
+       (Rmsg' "FieldAssign13 (single field rel)" ((#field_rel_single_tac basic_stmt_rel_info) ctxt) ctxt) THEN'
+       (Rmsg' "FieldAssign14 (Exp Rel Rhs)" (exp_rel_tac rcv_exp_rel_info ctxt) ctxt)
+
+    | _ => error "field assign rel tac only handles field assignment"
+    )
+
+  fun atomic_rel_inst_tac ctxt (basic_stmt_rel_info : basic_stmt_rel_info) (atomic_hint : atomic_rel_hint)  = 
+    (case atomic_hint of 
+        AssignHint (exp_wf_rel_info, exp_rel_info, lookup_bpl_target_thm) => 
+               red_assign_tac ctxt basic_stmt_rel_info exp_wf_rel_info exp_rel_info lookup_bpl_target_thm
+     |  FieldAssignHint _ => field_assign_rel_tac ctxt basic_stmt_rel_info atomic_hint
+    )
 \<close>
 
 end
